pulse/share/pulse/examples/parix/Promises.Examples3.fst
@@ -87,9 +87,9 @@ let is (i:iref) : invlist = [(inv_p <: vprop), i]
 
 let cheat_proof (i:iref)
   : (_:unit) ->
-      stt_ghost unit (invlist_names (is i))
-        (requires         invlist_inv (is i) ** (pts_to done #one_half true ** GR.pts_to claimed #one_half false))
-        (ensures fun _ -> invlist_inv (is i) ** (pts_to done #one_half true ** goal))
+      stt_ghost unit (add_inv emp_inames i)
+        (requires pts_to done #one_half true ** (inv i inv_p ** GR.pts_to claimed #one_half false))
+        (ensures fun _ -> pts_to done #one_half true ** goal)
   = admit() //proof is atomic, not ghost
 
 #set-options "--debug Promises.Examples3 --debug_level SMTQuery"
@@ -98,7 +98,8 @@ let cheat_proof (i:iref)
 fn setup (_:unit)
    requires pts_to done v_done ** pts_to res v_res ** GR.pts_to claimed v_claimed
    returns i:iref
-   ensures pts_to done #one_half false ** pledge (is i) (pts_to done #one_half true) goal
+   ensures pts_to done #one_half false **
+           pledge (add_inv emp_inames i) (pts_to done #one_half true) goal
 {
   done := false;
   res := None;
@@ -114,12 +115,12 @@ fn setup (_:unit)
   fold inv_p;
   
   let i = new_invariant inv_p;
-  rewrite (inv i inv_p ** emp) as (invlist_inv (is i));
+
   make_pledge
-    (is i)
+    (add_inv emp_inames i)
     (pts_to done #one_half true) //f
     goal  //v
-    (GR.pts_to claimed #one_half false)  //extra
+    (inv i inv_p ** GR.pts_to claimed #one_half false)  //extra
     (cheat_proof i);
 
   i
